Java/src/Logic/ProtocolLogic.v
@@ -53,37 +53,7 @@ Definition PM := Map [protocol, ST].
   Local Transparent BILPre_Ops.
   Local Transparent BILFun_Ops.
 
-  Definition pspec := PM -> spec.
-
-  Instance ILogicOpsPSpec    : ILogicOps pspec    := _.
-  Instance ILogicPSpec       : ILogic pspec       := _.
-  Instance ILLOperatorsPSpec : ILLOperators pspec := _.
-  (*Instance BILOperatorsPSpec : BILOperators pspec := _.
-  Instance BILogicPSpec      : BILogic pspec      := _.
-  Instance IBILogicPSasn     : IBILogic psasn     := _.*)
-
-  Instance EmbedPSpecPropOp : EmbedOp Prop pspec := _.
-  Instance EmbedPSpecProp   : Embed Prop pspec   := _.
-
-  Instance EmbedPSpecSpecOp : EmbedOp spec pspec := _.
-  Instance EmbedPSpecSpec   : Embed spec pspec   := _.
-
-  Program Definition prog_spec (X : Prog_wf -> Prop) : pspec :=
-    fun PM => mk_spec (fun (P : Prog_wf) _ => forall (Q : Prog_wf) , Prog_wf_sub P Q -> X Q) _ _.
-  Next Obligation.
-    intros; apply H0; etransitivity; eassumption.
-  Qed.
-
-  Notation "'[prog]' P"    := (prog_spec  P) (at level 65).
-
-
-  Program Definition ST_exists (p : protocol) (T : ST) : pspec :=
-    fun PM => mk_spec (fun P k =>
-      MapsTo p T PM
-    ) _ _.
-
-
-  Definition pasn := PM -> STs -> asn.
+  Definition pasn := STs -> asn.
   
   Instance ILogicOpsPAsn    : ILogicOps pasn    := _.
   Instance ILogicPAsn       : ILogic pasn       := _.
@@ -117,43 +87,28 @@ Definition PM := Map [protocol, ST].
   Instance EmbedPSasnSpecOp : EmbedOp spec psasn := _.
   Instance EmbedPSasnSpec   : Embed spec psasn   := _.
 
-  Instance EmbedPSasnPSpecOp : EmbedOp pspec psasn := _.
-  Instance EmbedPSasnPSpec   : Embed pspec psasn   := _.
-
   Instance EmbedPSasnAsnOp : EmbedOp asn psasn := _. 
   Instance EmbedPSasnAsn   : Embed asn psasn := _.
 
   Instance EmbedPSasnSasnOp : EmbedOp sasn psasn := _. 
   Instance EmbedPSasnSasn   : Embed sasn psasn := _.
   
-
-  Program Definition psasn_subst (P : psasn) (sub : subst) : psasn := 
-    fun s PM STs => mk_asn (fun Pr k h => P (stack_subst s sub) PM STs Pr k h) _ _ _.
-  Next Obligation.
-    solve_model H.
-  Defined.
-  Next Obligation.
-    solve_model H0.
-  Defined.
-  Next Obligation.
-    solve_model H0.
-  Defined.
-
   Program Definition has_ST (v : var) (T : ST) : psasn :=
-    fun s PM STs => mk_asn (fun P k h =>
+    fun s STs => mk_asn (fun P k h =>
       MapsTo (val_to_stptr (s v)) T STs
     ) _ _ _.
 
   Program Definition has_subst_ST (x z y : var) (T : ST) : psasn :=
-    fun s PM STs => mk_asn (fun P k h =>
+    fun s STs => mk_asn (fun P k h =>
       MapsTo (val_to_stptr (s x)) (subst_ST z (s y) T) STs
     ) _ _ _.
 
   Program Definition all_STs (T : ST) : psasn :=
-    fun s PM STs => mk_asn (fun P k h =>
+    fun s STs => mk_asn (fun P k h =>
       forall c, In c STs -> MapsTo c T STs
     ) _ _ _.
   
+  (*
   Import Marshall.
   Program Definition isMarshallable (v : var) (P : sasn) : psasn :=
   	fun s PM STs => mk_asn (fun Pr k h =>
@@ -168,7 +123,8 @@ Definition PM := Map [protocol, ST].
     eapply H0; [ | assumption | eassumption].
     transitivity h'; eassumption.
   Defined.
-
+  *)
+  
   (*
   Program Definition DecidableAsn (P : sasn) : sasn := 
     fun s => mk_asn (fun Pr n h =>
