Java/src/Logic/ST.v
@@ -3,7 +3,7 @@ Require Import RelationClasses Setoid Morphisms.
 Require Import MapInterface MapFacts.
 Require Import Open Stack Subst Lang OpenILogic Pure ILEmbed PureInsts.
 Require Import UUSepAlg SepAlgInsts.
-Require Import Heap AssertionLogic Util Program.
+Require Import Heap AssertionLogic Util Program Traces.
 
 Inductive ST : Type :=
   | st_end : ST
@@ -32,34 +32,13 @@ Fixpoint dual_ST (st : ST) : ST :=
   | st_recv v P st' => st_send v P (dual_ST st')
   end.
 
-Class Dual (A : Type) (dual : A -> A) : Prop := {
-  dual_involutive : forall a : A, dual (dual a) === a
-}.
-Definition dual {A : Type} {dual' : A -> A} {D : Dual A dual'} (a : A) : A := dual' a.
-Hint Unfold dual.
-
-Lemma dual_isomorphic_aux {A : Type} {dual' : A -> A} {D : Dual A dual'} : forall (a b : A), a === b -> dual a === dual b.
-Proof.
-  intros.
-  rewrite H; reflexivity.
-Qed.
-
-Lemma dual_isomorphic {A : Type} {dual' : A -> A} {D : Dual A dual'} : forall (a b : A), a === b <-> dual a === dual b.
-Proof.
-  split; intro H.
-  * apply dual_isomorphic_aux; assumption.
-  * apply dual_isomorphic_aux in H.
-    repeat rewrite dual_involutive in H.
-    assumption.
-Qed.
-
 Program Instance ST_Dual : Dual ST dual_ST := {
   dual_involutive := _
 }.
 Next Obligation.
   induction a; [ reflexivity | |];
   simpl; rewrite IHa; reflexivity.
-Qed.
+Defined.
 
 Fixpoint subst_ST (x : var) (v : val) (t : ST) : ST :=
   match t with
@@ -68,58 +47,18 @@ Fixpoint subst_ST (x : var) (v : val) (t : ST) : ST :=
   | st_recv x' A t' => st_recv x' (apply_subst A (subst1 `v x)) (subst_ST x v t')
   end.
 
-Module Marshall.
+Fixpoint ST_append (l r : ST) : ST :=
+  match l with
+    | st_end => r
+    | st_send v P l' => st_send v P (ST_append l' r)
+    | st_recv v P l' => st_recv v P (ST_append l' r)
+  end.
 
-
-	Inductive marshall (Pr : Prog_wf) (v : sval) (big : heap) : heap -> Prop :=
-	  | marshall_int  : forall (z : Z) (m : heap)
-	                       (Vint : v = vint z)
-	                   (Msubheap : subheap m big),
-	                   marshall Pr v big m
-	  | marshall_bool : forall (b : bool) (m : heap)
-	                       (Vbool : v = vbool b)
-	                    (Msubheap : subheap m big),
-	                    marshall Pr v big m
-	  | marshall_ptr  : forall (ref : ptr) (cls : class) (pos : nat) (m : heap) fields
-	                        (Vptr : v = vptr ref)
-	                      (Vclass : ref = (pos, cls))
-	                     (Vfields : field_lookup Pr cls fields)
-	                       (Mhere : forall (f : field) (v' : sval),
-	                                SS.In f fields ->
-	                                MapsTo (ref, f) v' (get_heap_ptr big) /\
-	                                MapsTo (ref, f) v' (get_heap_ptr m))
-	                      (Mchild : forall (f : field) (v' : sval),
-	                                SS.In f fields ->
-	                                MapsTo (ref, f) v' (get_heap_ptr big) ->
-	                                marshall Pr v' big m
-	                      ),
-	                     marshall Pr v big m.
-	   (*            
-	  | marshall_arr  : forall (ref : arrptr) (i : nat) (v' : sval) (m : heap)
-	                    (Varr : v = varr ref)
-	                    (Mmaps : MapsTo (ref, i) v' (get_heap_arr big))
-	                    (Mmarshalls : marshall v' big m),
-	                    marshall v big (heap_add_arr m ref i v')
-	.*)
-	
-	Lemma marshall_from_smaller {Pr : Prog_wf} {a b m : heap} {v : sval}
-	    (Hsubheap : subheap a b) (Hmarshall : marshall Pr v a m) :
-	    marshall Pr v b m.
-	Proof.
-	    induction Hmarshall.
-	    * eapply marshall_int; [eassumption | transitivity big; assumption].
-	    * eapply marshall_bool; [eassumption | transitivity big; assumption].
-	    * eapply marshall_ptr; try eassumption; intros f v' Hin; specialize (Mhere f v' Hin).
-	      + destruct Mhere as [Minput Mres].
-	        split; [| assumption].
-	        destruct Hsubheap as [? Hsubheap].
-	        eapply sa_mul_mapstoL; [apply Hsubheap | apply Minput].
-	      + intro Hinput.
-	        destruct Mhere as [Minput Mres].
-	        eapply H; eassumption.
-    Qed.
-
-End Marshall.
+Definition STs_append (l r : STs) : STs :=
+  mapi (fun k r' => match (find k l) with
+    | Some l' => ST_append l' r'
+    | None => r'
+    end) r. 
 
 Module STNotations.
   	(*Notation " x ':' t " := (has_ST x t) (at level 88, left associativity) : st_scope.*)
