Java/src/Logic/Traces.v
@@ -1,0 +1,83 @@
+Require Import RelationClasses Setoid Morphisms Coq.Classes.Equivalence.
+Require Import Lang Heap Rel Stack.
+Open Scope equiv_scope.
+
+Class Dual (A : Type) (dual : A -> A) : Prop := {
+  dual_involutive : forall a : A, dual (dual a) === a
+}.
+Definition dual {A : Type} {dual' : A -> A} {D : Dual A dual'} (a : A) : A := dual' a.
+Hint Unfold dual.
+
+Lemma dual_isomorphic_aux {A : Type} {dual' : A -> A} {D : Dual A dual'} : forall (a b : A), a === b -> dual a === dual b.
+Proof.
+  intros.
+  rewrite H; reflexivity.
+Qed.
+
+Lemma dual_isomorphic {A : Type} {dual' : A -> A} {D : Dual A dual'} : forall (a b : A), a === b <-> dual a === dual b.
+Proof.
+  split; intro H.
+  * apply dual_isomorphic_aux; assumption.
+  * apply dual_isomorphic_aux in H.
+    repeat rewrite dual_involutive in H.
+    assumption.
+Qed.
+
+Inductive trace : Type :=
+  | t_end   : trace
+  | t_send  : stptr -> val -> heap -> trace -> trace
+  | t_recv  : stptr -> val -> heap -> trace -> trace
+  | t_start : stptr -> trace -> trace -> trace
+  | t_tau : trace -> trace
+  .
+
+Fixpoint dual_trace (t : trace) : trace := 
+  match t with
+    | t_end => t_end
+    | t_start c t t' => t_start c t (dual_trace t')
+    | t_send c v h t' => t_recv c v h (dual_trace t')
+    | t_recv c v h t' => t_send c v h (dual_trace t')
+    | t_tau tr => t_tau (dual_trace tr)
+  end.
+
+Program Instance trace_Dual : Dual trace dual_trace := {
+  dual_involutive := _
+}.
+Next Obligation.
+  induction a; [ reflexivity | ..]; simpl; try rewrite IHa; try rewrite IHa2; reflexivity.
+Defined.
+
+Fixpoint trace_append (l r : trace) : trace :=
+  match l with
+    | t_end => r
+    | t_send c v h l' => t_send c v h (trace_append l' r)
+    | t_recv c v h l' => t_recv c v h (trace_append l' r)
+    | t_start c t l'  => t_start c t  (trace_append l' r)
+    | t_tau l' => t_tau (trace_append l' r)
+  end.
+  
+Fixpoint trace_length (l : trace) : nat :=
+  match l with
+    | t_end => O
+    | t_send _ _ _ l' => S (trace_length l')
+    | t_recv _ _ _ l' => S (trace_length l')
+    | t_start _ l' l'' => S (trace_length l') + (trace_length l'')
+    | t_tau l' => S (trace_length l')
+  end.
+
+Lemma trace_appendC : forall (a b c : trace), trace_append (trace_append a b) c = trace_append a (trace_append b c).
+Proof.
+  intros; induction a; simpl; try rewrite IHa; try rewrite IHa2; reflexivity.
+Qed.  
+
+Lemma trace_appendEndR : forall (a : trace), a = trace_append a t_end.
+Proof.
+  intros.
+  induction a; [reflexivity | ..]; simpl; try rewrite <- IHa; try rewrite <- IHa2; reflexivity.
+Qed.
+
+Lemma trace_appendLength : forall tr tr', trace_length (trace_append tr tr') >= trace_length tr.
+Proof.
+  intros; induction tr; intros; simpl; omega.
+Qed.
+  
