Java/src/Semantics/SemCmdRules.v
@@ -1,7 +1,7 @@
 Require Import SemCmd ILogic BILogic ILInsts BILInsts. 
 Require Import OpenILogic Later ProtocolLogic AssertionLogic SpecLogic ILEmbed Open.
 Require Import Stack Subst Lang Util Lists.List.
-Require Import FunctionalExtensionality ST.
+Require Import FunctionalExtensionality ST Traces.
 
 Set Implicit Arguments.
 Unset Strict Implicit.
@@ -28,19 +28,21 @@ Section Rules.
       (HPost : Q' |-- Q ) :
       {{P'}}c{{Q'}} |-- {{P}}c{{Q}}.
     Proof.
-      intros PM n Pr Hc Pr' m k s h t HPr Hmn Hkm HP; simpl.
-      destruct (Hc _ _ _ s h t HPr Hmn Hkm) as [HSafe HQ].
+      intros n Pr Hc Pr' m k s h cl pr HPr Hmn Hkm HP; simpl.
+      destruct (Hc _ _ _ s h cl pr HPr Hmn Hkm) as [HSafe HQ].
       + apply HPre; apply HP.
-      + split; [apply HSafe|intros t' h' s' H].
-        apply HPost. specialize (HQ _ _ _ H). apply HQ.
+      + split; [apply HSafe|intros tr h' s' cl' H].
+        eapply Comp_entails; [intros; apply HPost; apply H0 |].
+        specialize (HQ _ _ _ _ H). apply HQ.
     Qed.
 
 	Local Existing Instance EmbedPSasnSasnOp.
 
     Definition not_modifies (c : semCmd) (x : var) : Prop :=
-      forall PP PM s s' h h' STs STs' n (HSem : c PP PM n s h STs (Some (s', (h', STs')))),
+      forall PP s s' h h' cl cl' tr n (HSem : c PP n s h cl tr (Some (s', (h', cl')))),
         s x = s' x.
 
+    (*
     Lemma frame_rule : forall (P Q R : psasn) c (xs: list var)
       (HMod : forall x, ~ In x xs -> not_modifies c x),
       {{ P }} c {{ Q }} |--
@@ -48,50 +50,70 @@ Section Rules.
     Proof.
       intros.
       (* Should have something with [T1 T2 TSub], where (T1 T2 : STs) and (TSub: sa_mul T1 T2 STs) *)
-      intros PM PP n HSpec PP' ? ? ? ? STs HPP' Hmn Hkm [h1 [h2 [HSub [HP HR]]]]; split.
+      intros PP n HSpec PP' ? ? ? ? ? pr HPP' Hmn Hkm [h1 [h2 [HSub [HP HR]]]]; split.
       (* safety *)
-      { destruct (HSpec _ m k s h STs HPP' Hmn Hkm) as [HS _]; [ | assumption].
+      { destruct (HSpec _ m k s h cl pr HPP' Hmn Hkm) as [HS _]; [ | assumption].
         solve_model HP. exists h2; apply HSub.
       }
       (* correctness *)
-      intros ? ? ? HSem. 
+      intros ? ? ? ? HSem. 
+      
       (* Should be given STs STs' T2 T1 instead *)
-      destruct (@cmd_frame c PP' PM s s' h h' h2 h1 k STs STs' (MapInterface.empty _) STs ) as [h'' [t'' [HBig [TBig Hc]]]]. 
+      destruct (@cmd_frame c PP' s s' h h' h2 h1 cl cl' k tr) as [h'' [HBig Hc]]. 
       + assumption.
-      + apply UUSepAlg.uusa_unit; apply MapInterface.empty_1.
       + intros l Hle.
-        destruct (HSpec _ m l s h1 STs HPP' Hmn) as [HS _]; [ omega | assumption |].
-        apply HS.
+        destruct (HSpec _ m l s h1 pr HPP' Hmn) as [HS _]; [ omega | solve_model HP; exists h2; assumption | ].
+        intros ? ? Htr Hfail.
+        specialize (HS _ _ Hfail).
+        admit (* fangel, used, frame-rule, oh-boy-safety-fun *).
+        (*
+        rewrite Htr in HSem.
+        clear HP HR Hfail Htr. generalize dependent pr. generalize dependent tr. generalize dependent tr''.
+        induction tr'; intros tr'' HSem tr pr HS; simpl in HS; [ apply HS; reflexivity | ..].
+        remember (MapInterface.find s0 pr ); destruct o; [| assumption]; destruct s1; try assumption; destruct HS as [_ HS].
+        specialize (IHtr' _ _ HSem Htr).
+        
+        
+        destruct (HSpec _ m k s h pr HPP' Hmn) as [_ HComp]; [ omega | solve_model HP; exists h2; assumption | ].
+        specialize (HComp _ _ _ HSem).
+        assert (c PP' k s h1 tr (Some (s', h'))) by admit (* fangel, used, test *).
+        specialize (HS tr (Some (s', h')) _ Hle H).
+        
+        apply HS. *)
       + assumption.
       + (* should be T1 instead of STs *)
-        destruct (HSpec _ m k s h1 STs HPP' Hmn Hkm) as [_ HC]. 
+        destruct (HSpec _ m k s h1 pr HPP' Hmn Hkm) as [_ HC]. 
         * apply HP.
         * specialize (HC _ _ _ Hc).
+          eapply Comp_entails; [| apply HC].
+          intros.
           exists h'', h2, HBig.
-          (* should have an exists T'', T2, TBig *) 
-          split; [solve_model HC; admit (* fangel, used *) |].
+          split; [apply H |].
           simpl. exists s. unfold apply_subst, id.
-          simpl in HR; unfold id in HR. 
+          simpl in HR. 
           solve_model HR.
-          - admit (* fangel, used *).
+          - admit (* fangel, used, frame-rule *).
           - apply functional_extensionality. intros x.
             unfold stack_subst, subst_fresh.
             destruct (in_dec Rel.dec_eq x xs) as [|HNotIn]; [reflexivity|].
             unfold not_modifies in HMod. 
-            specialize (HMod _ HNotIn _ PM _ _ _ _ _ _ _ HSem).
+            specialize (HMod _ HNotIn _ _ _ _ _ _ _ HSem).
             apply HMod.
     Qed.
-
+    *)
+    
     Lemma conj_rule G P1 P2 Q1 Q2 c 
       (H1 : G |-- {{P1}} c {{Q1}})
       (H2 : G |-- {{P2}} c {{Q2}}) :
       G |-- {{P1 //\\ P2}} c {{Q1 //\\ Q2}}.
     Proof.
-      intros PM n P HPP HG.
-      simpl. intros m k s h STs HPP' Hm Hk [HP1 HP2]. split.
+      intros n P HPP HG.
+      simpl. intros m k s h cl pr HPP' Hm Hk [HP1 HP2]. split.
       + eapply H1; eauto.
-      + intros STs' h' s' Hsem.
-        split; [eapply H1|eapply H2]; eauto.
+      + intros tr h' s' cl' Hsem.
+        specialize (H1 _ _ HPP); specialize (H1 _ _ _ _ _ cl _ HPP' Hm Hk HP1); destruct H1 as [_ H1]; specialize (H1 _ _ _ _ Hsem).
+        specialize (H2 _ _ HPP); specialize (H2 _ _ _ _ _ cl _ HPP' Hm Hk HP2); destruct H2 as [_ H2]; specialize (H2 _ _ _ _ Hsem).
+        eapply Comp_split; eassumption.
     Qed.
 
   End StructuralRules.
@@ -100,119 +122,142 @@ Section Rules.
 
     Lemma skip_rule P : |-- {{P}}skip_cmd {{P}}.
     Proof.
-      intros PM n Pr HPP Pr' m k s h STs _ Hmn Hkm HP; split.
-      + intros H; inversion H.
-      + intros STs' h' s' HSem; inversion HSem; subst.
+      intros n Pr HPP Pr' m k s h cl pr _ Hmn Hkm HP; split.
+      + intros tr cfg H; inversion H; subst; congruence.
+      + intros tr h' s' cl' HSem; inversion HSem; subst; simpl.
         solve_model HP.
     Qed.
 
     Lemma seq_rule c1 c2 P Q R :
       ({{P}}c1{{Q}} //\\ {{Q}}c2{{R}}) |-- {{P}}seq_cmd c1 c2{{R}}.
     Proof.
-      intros PM Pr n [Hc1 Hc2] Pr' k m s h STs HPP' Hmn Hkm HP; split.
-      + intros HFail; inversion HFail; subst; clear HFail.	
-        * destruct (Hc1 _ _ n0 s h STs HPP' Hmn) as [HS _];
-          [omega | assumption | apply HS; assumption ].
-        * destruct (Hc1 _ _ n0 s h STs HPP' Hmn) as [_ HC]; [omega | assumption |].
-          specialize (HC _ _ _ H).
-          destruct (Hc2 _ (k - n0) n' s' h' STs' HPP') as [HS _]; [omega | omega | |].
-          apply HC. 
-          apply HS; exact H0.
-      + intros STs' h' s' HSem; inversion HSem; subst; clear HSem.
-        destruct (Hc1 _ _ n0 s h STs HPP' Hmn) as [_ HC1]; [omega | assumption |].
-        specialize (HC1 _ _ _ H7).
-        destruct (Hc2 _ (k - n0) n1 s1 h1 STs1 HPP') as [_ HC2]; [omega | omega | |].
-        apply HC1.
-        specialize (HC2 _ _ _ H9).
-        solve_model HC2. 
+      intros Pr n [Hc1 Hc2] Pr' k m s h cl pr HPP' Hmn Hkm HP; split.
+      + intros tr cfg H. destruct cfg.  
+        * inversion H; subst; clear H.
+          destruct (Hc1 _ _ n0 s h cl pr HPP' Hmn) as [_ HC1]; [omega | solve_model HP |]; specialize (HC1 _ _ _ _ H1).
+          assert (n0 = trace_length tr0) by admit (* fangel, fuel = trace-length *).
+          eapply Comp_partial; [eassumption | eassumption | apply HC1 |].
+          intros; simpl in H0.
+          destruct (Hc2 _ n1 n1 s1 h1 cl1 pr0 HPP') as [_ HC2]; [omega | omega | solve_model H0 |]; specialize (HC2 _ _ _ _ H8).
+          eapply Comp_entails; [congruence | apply HC2].
+        * inversion H; subst; clear H.
+          - destruct (Hc1 _ _ m s h cl pr HPP' Hmn) as [HS _]; [omega | assumption |]; specialize (HS _ _ H0); assumption.
+          - destruct (Hc1 _ _ n0 s h cl pr HPP' Hmn) as [_ HC1]; [omega | solve_model HP |]; specialize (HC1 _ _ _ _ H0).
+            assert (n0 = trace_length tr0) by admit (* fangel, fuel = trace-length *).
+            eapply Comp_partial; [ eassumption | eassumption | apply HC1 |].
+            intros; simpl in H.
+            destruct (Hc2 _ n' n' s' h' cl' pr0 HPP') as [HS _]; [omega | omega | solve_model H2 |]; specialize (HS _ _ H1); assumption.
+      + intros tr h' s' cl' HSem; inversion HSem; subst; clear HSem.
+        destruct (Hc1 _ _ n0 s h cl pr HPP' Hmn) as [_ HC1]; [omega | solve_model HP |]; specialize (HC1 _ _ _ _ H7).
+        assert (n0 = trace_length tr0) by admit (* fangel, fuel = trace-length *).
+        eapply Comp_partial; [ eassumption | eassumption | apply HC1 |].
+        intros; simpl in H.
+        destruct (Hc2 _ n1 n1 s1 h1 cl1 pr0 HPP') as [_ HC2]; [omega | omega | solve_model H0 |]; specialize (HC2 _ _ _ _ H9).
+        eapply Comp_entails; [| apply HC2].
+        intros; simpl in H0.
+        solve_model H1.
     Qed.
 
     Lemma nondet_rule c1 c2 P Q:
       ({{P}}c1{{Q}} //\\ {{P}}c2{{Q}}) |-- {{P}}nondet_cmd c1 c2{{Q}}.
     Proof.
-      intros PM n Pr [Hc1 Hc2] Pr' k m s h STs HPP' Hmn Hkm HP; split.
-      + intros HFail; inversion HFail; subst; clear HFail.
-        * destruct (Hc1 _ _ n0 s h STs HPP' Hmn) as [HS _];
-          [omega | assumption | apply HS; assumption].
-        * destruct (Hc2 _ _ n0 s h STs HPP' Hmn) as [HS _];
-          [omega | assumption | apply HS; assumption].
-      + intros h1 s1 STs1 HSem; inversion HSem; subst; clear HSem.
-        * destruct (Hc1 _ _ n0 s h STs HPP' Hmn) as [_ HC]; [omega | assumption |].
-          specialize (HC _ _ _ H6). 
-          solve_model HC.
-        * destruct (Hc2 _ _ n0 s h STs HPP' Hmn) as [_ HC]; [omega | assumption |].
-          specialize (HC _ _ _ H6).
-          solve_model HC.
+      intros n Pr [Hc1 Hc2] Pr' k m s h cl pr HPP' Hmn Hkm HP; split.
+      + intros tr cfg Hsem.
+        destruct cfg; inversion Hsem; subst.
+        * destruct (Hc1 _ _ m s h cl pr HPP' Hmn) as [HS _]; [omega | assumption |]; specialize (HS _ _ H6); assumption.
+        * destruct (Hc2 _ _ m s h cl pr HPP' Hmn) as [HS _]; [omega | assumption |]; specialize (HS _ _ H6); assumption.
+        * destruct (Hc1 _ _ m s h cl pr HPP' Hmn) as [HS _]; [omega | assumption |]; specialize (HS _ _ H).
+          induction tr; simpl; simpl in HS; [congruence | | | apply HS | auto];
+          (remember (MapInterface.find s0 pr); destruct o; [| assumption]; destruct s1; assumption).
+        * destruct (Hc2 _ _ m s h cl pr HPP' Hmn) as [HS _]; [omega | assumption |]; specialize (HS _ _ H).
+          induction tr; simpl; simpl in HS; [congruence | | | apply HS | auto];
+          (remember (MapInterface.find s0 pr); destruct o; [| assumption]; destruct s1; assumption).
+      + intros tr h1 s1 cl1 HSem; inversion HSem; subst; clear HSem.
+        * destruct (Hc1 _ _ m s h cl pr HPP' Hmn) as [_ HC]; [omega | assumption |]; specialize (HC _ _ _ _ H6).
+          eapply Comp_entails; [| apply HC].
+          intros; simpl in H; solve_model H. 
+        * destruct (Hc2 _ _ m s h cl pr HPP' Hmn) as [_ HC]; [omega | assumption |]; specialize (HC _ _ _ _ H6).
+          eapply Comp_entails; [| apply HC].
+          intros; simpl in H; solve_model H. 
     Qed.
 
     Lemma kleene_rule c P:
       {{P}}c{{P}} |-- {{P}} kleene_cmd c {{P}}.
     Proof.
-      intros PM Pr n Hc Pr' m k s h STs HPP' Hmn Hkm Hp; split.
-      + intros HFail. generalize dependent m. remember None as cfg.
-        induction HFail; intros; inversion Heqcfg; subst.
-        * destruct (Hc _ m n0 s h STs HPP' Hmn) as [HS _];
-          [omega | assumption | apply HS; assumption].
-        * destruct (Hc _ m n0 s h STs HPP' Hmn) as [_ HC]; [omega | assumption |].
-          apply IHHFail with (m-n0); [assumption | assumption| reflexivity | omega | omega | ].
-          specialize (HC _ _ _ H).
-          solve_model HC.
-      + intros. remember (Some (s', (h', STs'))) as cfg. generalize dependent m. 
+      intros Pr n Hc Pr' m k s h cl pr HPP' Hmn Hkm Hp; split.
+      + intros tr cfg HSem.
+        generalize dependent pr. generalize dependent m.
+        induction HSem; simpl; intros.
+        - congruence.
+        - destruct (Hc _ m n0 s h cl pr HPP' Hmn Hkm Hp) as [HS _]. 
+          apply HS; assumption.
+        - assert (n0 = trace_length tr) by admit (* fangel, trace-length *).
+          destruct (Hc _ _ n0 s h cl pr HPP' Hmn) as [_ HC]; [omega | solve_model Hp |]; specialize (HC _ _ _ _ H).
+          eapply Comp_partial; [ eassumption | eassumption | apply HC |]. 
+          intros. simpl in H1.
+          eapply IHHSem; [ assumption | | reflexivity | apply H1]; omega.
+        - assert (n0 = trace_length tr) by admit (* fangel, trace-length *).
+          destruct (Hc _ _ n0 s h cl pr HPP' Hmn) as [_ HC]; [omega | solve_model Hp |]; specialize (HC _ _ _ _ H).
+          eapply Comp_partial; [ eassumption | eassumption | apply HC |].
+          intros. simpl in H1.
+          eapply IHHSem; [ assumption | | reflexivity | apply H1]; omega.
+      + intros. remember (Some (s', (h', cl'))) as cfg. generalize dependent m. generalize dependent pr.
         induction H; inversion Heqcfg; subst; intros.
-        * solve_model Hp.
-        * destruct (Hc _ m n0 s h STs HPP' Hmn) as [_ HC]; [omega | assumption |].
-          specialize (HC _ _ _ H).
-          assert ((((P s' PM STs') Pr0) ((m - n0) - n1)) h') as H2. 
-            apply IHkleene_sem; try assumption; try omega. 
-          solve_model H2.
+        * simpl. solve_model Hp.
+        * assert (n0 = trace_length tr) by admit (* fangel, trace-length *).
+          destruct (Hc _ _ n0 s h cl pr HPP' Hmn) as [_ HC]; [omega | assumption |].
+          specialize (HC _ _ _ _ H).
+          eapply Comp_partial; [ eassumption | eassumption | apply HC |].
+          intros. simpl in H2.
+          apply IHkleene_sem; [ assumption | reflexivity | | reflexivity | apply H2]; omega.
     Qed.
-
+    
     Lemma assume_rule P (t : vlogic) :
       |-- {{P}} assume_cmd t {{t /\\ P}}.
     Proof.
-      intros PM n Pr Hc Pr' m k s h STs HPP' Hmn Hkm Hp; split.
-      + intros HFail. inversion HFail.
-      + intros STs' h' s' H. remember (Some (s', (h', STs'))) as cfg; induction H.
-        inversion Heqcfg; subst; intros.
+      intros n Pr Hc Pr' m k s h cl pr HPP' Hmn Hkm Hp; split.
+      + intros; inversion H; subst; simpl. congruence.
+      + intros tr' h' s' cl' H. remember (Some (s', (h', cl'))) as cfg; induction H; simpl.
+        inversion Heqcfg; subst; clear Heqcfg; intros.
         split; [assumption|]. solve_model Hp.
     Qed.
 
     Lemma assert_rule (P : psasn) (p : vlogic) (HPe : P |-- embed p) :
       |-- {{P}} assert_cmd p {{P}}.
     Proof.
-      intros PM n Pr Hc Pr' m k s h STs HPP' Hmn Hkm Hp; specialize (HPe _ _ _ _ _ _ Hp); split.
-      + intros HF; inversion HF; subst; auto.
-      + intros STs' h' s' HSem; inversion HSem; subst.
+      intros n Pr Hc Pr' m k s h cl pr HPP' Hmn Hkm Hp; specialize (HPe _ _ _ _ _ Hp); split.
+      + intros; inversion H; subst; simpl; [ congruence | auto].
+      + intros tr h' s' cl' HSem; inversion HSem; subst; simpl.
         solve_model Hp.
     Qed.
-
+    
   End PrimitivesRules.
 
   Lemma exists_into_precond {A} (P: A -> psasn) c q :
     (Forall x, {{P x}} c {{q}}) -|- {{Exists x, P x}} c {{q}}.
   Proof.
   	split.
-  	+ intros PM n Pr Hp Pr' m k s h STs HPP' Hmn Hkm [x Hxp]; specialize (Hp x); auto.
-  	+ intros PM n Pr Hp x Pr' m k s h STs HPP' Hmn Hkm Hxp.
+  	+ intros n Pr Hp Pr' m k s h cl pr HPP' Hmn Hkm [x Hxp]; specialize (Hp x); auto.
+  	+ intros n Pr Hp x Pr' m k s h cl pr HPP' Hmn Hkm Hxp.
   	  apply Hp; try assumption. exists x; apply Hxp.
   Qed.
 
   (* Holds only in one direction unless annotations on assertion logic, which is ugly - well, it's happened. - F.
      This is the important direction, though *)
-  Lemma I_precond (SP : pspec) (P Q : psasn) c:
+  Lemma I_precond (SP : spec) (P Q : psasn) c:
     (SP -->> {{ P }} c {{ Q }}) -|- {{ SP /\\  P }} c {{ Q }}.
   Proof.
   	split.
-  	+ intros PM Pr n Hp Pr' m k s h STs HPP' Hmn Hkm [HSP HP].
+  	+ intros Pr n Hp Pr' m k s h cl pr HPP' Hmn Hkm [HSP HP].
   	  specialize (Hp Pr' HPP' m Hmn HSP).
   	  apply Hp; reflexivity || assumption.
-  	+ intros PM Pr n Hp Pr' HPP' m Hnm HSP Pr'' k l s h STs HPP'' Hkm Hkl HP.
+  	+ intros Pr n Hp Pr' HPP' m Hnm HSP Pr'' k l s h cl pr HPP'' Hkm Hkl HP.
   	  apply Hp.
   	  * transitivity Pr'; assumption.
   	  * omega.
   	  * omega.
   	  * simpl. split. 
-        assert ((SP PM Pr'') k). solve_model HSP. intros a b. simpl. intuition.
+        assert ((SP Pr'') k). solve_model HSP. intros a b. simpl. intuition.
         apply H. apply HP.
   Qed.
 
